TransClosure.v
@@ -1,0 +1,23 @@
+Require Import Lists.List.
+Require Import Coq.Relations.Relations.
+
+Section REL_DEC.
+
+Variable A: Type.
+
+Variable R: A -> A -> Prop.
+
+Variable pairs : list (A * A) % type.
+
+Lemma clos_trans_dec (rel_spec: forall x y,
+  R x y <-> In (x, y) pairs):
+  forall x y,
+  { clos_trans A R x y } + { ~ clos_trans A R x y }.
+Proof.
+  intros.
+  destruct pairs.
+  - 
+  assert (Hx := rel_spec x y).
+Admitted.
+
+End REL_DEC.
